

$$\begin{array}{c}
 Q_a(\partial B) \\
 \uparrow \\
 \mathcal{O}(x) \\
 \bullet
 \end{array}
 =
 \begin{array}{c}
 \leftarrow \\
 \leftarrow \\
 \leftarrow \\
 \bullet \\
 \leftarrow \\
 \leftarrow \\
 \leftarrow
 \end{array}
 \begin{array}{c}
 \rightarrow \\
 \rightarrow \\
 \rightarrow \\
 \bullet \\
 \rightarrow \\
 \rightarrow \\
 \rightarrow
 \end{array}
 =
 \begin{array}{c}
 \leftarrow \\
 \leftarrow \\
 \leftarrow \\
 Q_a \mathcal{O}(x) \bullet \\
 \leftarrow \\
 \leftarrow \\
 \leftarrow
 \end{array}
 -
 \begin{array}{c}
 \leftarrow \\
 \leftarrow \\
 \leftarrow \\
 \mathcal{O}(x) \bullet \\
 \leftarrow \\
 \leftarrow \\
 \leftarrow
 \end{array}
 Q_a
 =
 \begin{array}{c}
 \bullet \\
 \bullet \\
 \bullet \\
 \bullet \\
 \bullet \\
 \bullet \\
 \bullet
 \end{array}$$